Sebastian wanted an oracle

theories/Spilling/SplitSpill.v
@@ -10,8 +10,17 @@ Set Implicit Arguments.
 
 (** * SplitSpill *)
 
+Class kill_oracle_spec (kill_oracle:nat -> set var -> set var) :=
+  {
+    kill_oracle_incl : forall k (X:set var), kill_oracle k X ⊆ X;
+    kill_oracle_card : forall k X, cardinal X >= k -> cardinal (kill_oracle k X) = k;
+    kill_oracle_idem : forall k X, cardinal X < k -> kill_oracle k X [=] X
+  }.
 
-Fixpoint splitSpill
+Section KO.
+  Variable (kill_oracle:nat -> set var -> set var).
+
+Fixpoint splitSpillKO
          (k : nat)
          (ZL: list params)
          (Λ : list (⦃var⦄ * ⦃var⦄))
@@ -22,49 +31,54 @@ Fixpoint splitSpill
   : spilling :=
   match s,Lv with
 
-  | stmtLet x e s, ann1 LV lv
+  | stmtLet x e s, ann1 lv lvs
     => let Fv_e := Exp.freeVars e in
-       let L    := Fv_e \ R in
-       let K    := of_list (take (cardinal L) (elements (R \ Fv_e))) in
-       let R_e  := R \ K ∪ L in
+      let R := R ∩ lv in
+      let L    := Fv_e \ R in
+      let K    := kill_oracle (cardinal L - (k - cardinal R)) (R \ Fv_e) in
+      let R_e  := R \ K ∪ L in
 
-       let K_x  := one_or_empty_if k R_e in
-       let Sp   := getAnn lv ∩ (K ∪ K_x) \ M in
-       let R_s  := {x; R_e \ K_x} in
+      let K_x  := one_or_empty_if k R_e in
+      let Sp   := getAnn lvs ∩ (K ∪ K_x) \ M in
+      let R_s  := {x; R_e \ K_x} in
 
-       ann1 (Sp,L,nil) (splitSpill k ZL Λ R_s (Sp ∪ M) s lv)
+      ann1 (Sp,L,nil) (splitSpillKO k ZL Λ R_s (Sp ∪ M) s lvs)
 
-  | stmtReturn e, _
+  | stmtReturn e, ann0 lv
     => let Fv_e := Op.freeVars e in
+      let R := R ∩ lv in
        let L    := Fv_e \ R in
-       let K    := of_list (take (cardinal L) (elements (R \ Fv_e))) in
+       let K    := kill_oracle (cardinal L - (k - cardinal R)) (R \ Fv_e) in
        let R_e  := R \ K ∪ L in
        let Sp   := ∅ in
 
        ann0 (Sp,L,nil)
 
-  | stmtIf e s1 s2, ann2 LV lv1 lv2
+  | stmtIf e s1 s2, ann2 lv lv1 lv2
     => let Fv_e := Op.freeVars e in
+      let R := R ∩ lv in
        let L    := Fv_e \ R in
-       let K    := of_list (take (cardinal L) (elements (R \ Fv_e))) in
+       let K    := kill_oracle (cardinal L - (k - cardinal R)) (R \ Fv_e) in
        let R_e  := R \ K ∪ L in
        let Sp   := (getAnn lv1 ∪ getAnn lv2) ∩ K in
 
-       ann2 (Sp,L,nil) (splitSpill k ZL Λ R_e (Sp ∪ M) s1 lv1)
-            (splitSpill k ZL Λ R_e (Sp ∪ M) s2 lv2)
+       ann2 (Sp,L,nil) (splitSpillKO k ZL Λ R_e (Sp ∪ M) s1 lv1)
+            (splitSpillKO k ZL Λ R_e (Sp ∪ M) s2 lv2)
 
-  | stmtApp f Y, _
+  | stmtApp f Y, ann0 lv
     => let R_f := fst (nth (counted f) Λ (∅,∅)) in
-       let M_f := snd (nth (counted f) Λ (∅,∅)) in
+      let M_f := snd (nth (counted f) Λ (∅,∅)) in
+      let R := R ∩ lv in
        let Z   := nth (counted f) ZL nil in
        let L   := R_f \ R \ of_list Z in
-       let K    := of_list (take (cardinal L) (elements (R \ R_f))) in
+       let K    := kill_oracle (cardinal L - (k - cardinal R)) (R \ R_f) in
        let Sp   := M_f \ M \ of_list Z ∪ (((list_union (Op.freeVars ⊝ Y) \ M) ∩ K)) in
 
        ann0 (Sp,L, (R \ K ∪ L, list_union (Op.freeVars ⊝ Y) \ (R \ K ∪ L))::nil)
 
   | stmtFun F t, annF LV als lv_t
-    => let rms:= (fun f al =>
+    =>
+    let rms:= (fun f al =>
                    let Lv  := getAnn al in (* liveness in fn body *)
                    let Z  := fst f in    (* params of fn *)
                    let R_f := of_list (take k (elements Lv)) in
@@ -78,10 +92,10 @@ Fixpoint splitSpill
        annF (∅, ∅, rms)
             ((fun f rmlv
               => match rmlv with (rm, Lv)
-                                => splitSpill k ZL' Λ' (fst rm) (snd rm) (snd f) Lv
+                                => splitSpillKO k ZL' Λ' (fst rm) (snd rm) (snd f) Lv
                  end)
                ⊜ F ((fun rm al => (rm,al)) ⊜ rms als))
-            (splitSpill k ZL' Λ' R M t lv_t)
+            (splitSpillKO k ZL' Λ' R M t lv_t)
 
   | _,_ => ann0 (∅, ∅, nil)
 
@@ -115,152 +129,118 @@ Proof.
 cset_tac.
 Qed.
 
-Lemma fTake X `{OrderedType X} (s t : set X) n
- : t ⊆ (s \ of_list (take n (elements (s \ t))) ∪ t \ s).
+Variable kos : kill_oracle_spec kill_oracle.
+
+Lemma kill_oracle_incl2 (s t : set var) n
+ : t ⊆ (s \ kill_oracle n (s \ t)) ∪ t \ s.
 Proof.
-  assert (of_list (take n (elements ( s \ t))) ⊆ s \ t) as takeIncl. {
-    rewrite take_set_incl. eauto with cset.
-  }
-  apply incl_minus_incl with (u:=s) in takeIncl.
-  rewrite <- takeIncl.
-  rewrite seteq at 1.
-  reflexivity.
+  rewrite kill_oracle_incl. cset_tac.
 Qed.
 
 
-Lemma rke X `{OrderedType X} (s t: set X) (k : nat)
-: cardinal s <= k ->
-  cardinal t <= k ->
-  cardinal (s \ of_list (take (cardinal (t \ s)) (elements (s \ t))) ∪ t \ s) <= k.
+Lemma omega_help1 X k Y
+ : X - (k - Y) <= Y
+   ->  Y <= k
+   -> X + (Y - (X - (k - Y))) <= k.
 Proof.
-set (K := of_list (take (cardinal (t \ s)) (elements (s \ t)))) in *.
-decide (cardinal (t \ s) <= cardinal (s \ t)).
-* assert (cardinal K = cardinal (t \ s)) as crdKL.
-  { subst K. rewrite <- elements_length.
-    rewrite elements_of_list_size.
-    + rewrite take_length_le; eauto. rewrite elements_length. eauto.
-    + apply take_dupFree.
-  }
- rewrite union_cardinal_le. rewrite cardinal_difference'.
-  + rewrite crdKL.
-    decide (cardinal (t \ s) <= cardinal s).
-    - rewrite plus_comm.
-      rewrite <- le_plus_minus; eauto. (* uses RleqK *)
-    - rewrite not_le_minus_0.
-      ** simpl. rewrite cardinal_difference. eauto.
-      ** eauto.
-  + subst K. rewrite take_set_incl. eauto with cset.
-* apply not_le in n. subst K. rewrite take_eq_ge.
-  + rewrite of_list_elements. rewrite minus_minus.
-    enough (s ∩ t ∪ t \ s [=] t).
-    { rewrite H0. eauto. }
-    clear. cset_tac.
-  + clear - n. rewrite elements_length. omega.
+  omega.
 Qed.
 
-Lemma rke' X `{OrderedType X} (s t u: set X) (k : nat)
+Lemma rke (s t: set var) (k : nat)
 : cardinal s <= k ->
   cardinal t <= k ->
-  cardinal (s \ of_list (take (cardinal (t \ s \ u)) (elements (s \ t))) ∪ t \ s \ u) <= k.
+  cardinal (s \ kill_oracle (cardinal (t \ s) -(k - cardinal s)) (s \ t) ∪ t \ s) <= k.
 Proof.
-set (K := of_list (take (cardinal (t \ s \ u)) (elements (s \ t)))) in *.
-decide (cardinal (t \ s \ u) <= cardinal (s \ t)).
-* assert (cardinal K = cardinal (t \ s \ u)) as crdKL.
-  { subst K. rewrite <- elements_length.
-    rewrite elements_of_list_size.
-    + rewrite take_length_le; eauto. rewrite elements_length. eauto.
-    + apply take_dupFree.
+set (K := kill_oracle (cardinal (t \ s)-(k - cardinal s)) (s \ t)) in *.
+decide (cardinal (t \ s) - (k - cardinal s) <= cardinal (s \ t)).
+- assert (cardinal K = cardinal (t \ s)-(k - cardinal s)) as crdKL.
+  { subst K. rewrite kill_oracle_card; eauto.
   }
- rewrite union_cardinal_le. rewrite cardinal_difference'.
+  rewrite union_cardinal_le. rewrite cardinal_difference'.
   + rewrite crdKL.
-    decide (cardinal (t \ s \ u) <= cardinal s).
-    - rewrite plus_comm.
-      rewrite <- le_plus_minus; eauto.
-    - rewrite not_le_minus_0.
-      ** simpl. intros.
+    decide (cardinal (t \ s) - (k - cardinal s) <= cardinal s).
+    * rewrite plus_comm.
+      intros. eapply omega_help1; eauto.
+    * rewrite not_le_minus_0.
+      -- simpl. rewrite cardinal_difference. eauto.
+      -- eauto.
+  + subst K. rewrite kill_oracle_incl. eauto with cset.
+- apply not_le in n. subst K.
+  rewrite kill_oracle_idem; eauto.
+  rewrite minus_minus.
+  assert (EQ:s ∩ t ∪ t \ s [=] t) by cset_tac.
+  rewrite EQ; eauto.
+Qed.
+
+Lemma rke' (s t u: set var) (k : nat)
+: cardinal s <= k ->
+  cardinal t <= k ->
+  cardinal (s \ kill_oracle (cardinal (t \ s \ u) -(k - cardinal s)) (s \ t) ∪ t \ s \ u) <= k.
+Proof.
+set (K := kill_oracle (cardinal (t \ s \ u) -(k - cardinal s) ) (s \ t)) in *.
+decide (cardinal (t \ s \ u) -(k - cardinal s) <= cardinal (s \ t)).
+- assert (cardinal K = cardinal (t \ s \ u) -(k - cardinal s)) as crdKL.
+  { subst K.
+    rewrite kill_oracle_card; eauto.
+  }
+  rewrite union_cardinal_le. rewrite cardinal_difference'.
+  + rewrite crdKL.
+    decide (cardinal (t \ s \ u) - (k - cardinal s) <= cardinal s).
+    * rewrite plus_comm.
+      intros. eapply omega_help1; eauto.
+    * rewrite not_le_minus_0.
+      -- simpl. intros.
          rewrite !cardinal_difference. eauto.
-      ** intro. eauto.
-  + subst K. rewrite take_set_incl. eauto with cset.
-* apply not_le in n. subst K. rewrite take_eq_ge.
-  + rewrite of_list_elements. rewrite minus_minus.
-    enough (s ∩ t ∪ t \ s \ u [=] t \ (u \ s ∩ t)).
-    { rewrite H0. intros; rewrite cardinal_difference; eauto. }
-    clear. cset_tac.
-  + clear - n. rewrite elements_length. omega.
+      -- intro. eauto.
+  + subst K. rewrite kill_oracle_incl. eauto with cset.
+- apply not_le in n. subst K.
+  rewrite kill_oracle_idem; eauto.
+  rewrite minus_minus.
+  enough (s ∩ t ∪ t \ s \ u [=] t \ (u \ s ∩ t)).
+  { rewrite H. intros; rewrite cardinal_difference; eauto. }
+  clear. cset_tac.
 Qed.
 
-Lemma rkk X `{OrderedType X} (s t  : set X) (k : nat) (x y : X)
-: let K :=  of_list (take
-                       (cardinal (t \ s))
-                       (elements (s \ t))
-                  ) in
+Lemma rkk (s t  : set var) (k : nat) (x : var)
+: let K :=  kill_oracle (cardinal (t \ s) - (k - cardinal s)) (s \ t) in
   let  K_x := one_or_empty_if k (s \ K ∪ t \ s) in
    cardinal s <= k
 -> cardinal (t) <= k
 -> k > 0
 -> cardinal (s \ K ∪ t \ s) >= k
-
 -> cardinal {x; (s \ K ∪ t \ s) \ K_x} <= k.
 Proof.
 intros K K_x RleqK fvBcard kgeq1 sizeRL.
 rewrite add_cardinal. rewrite cardinal_difference'.
 - subst K_x. rewrite one_or_empty_cardinal_ge.
-  assert (rke := @rke X _ s t k RleqK fvBcard).
+  assert (rke := @rke s t k RleqK fvBcard).
   remember (cardinal (s \ K ∪ t \ s)).
   destruct n.
   + omega. (*uses kgt0*)
   + simpl.
-    enough (S n <= k). { omega. } rewrite Heqn. subst. exact rke.
+    enough (S n <= k). { omega. } rewrite Heqn. subst.
+    eapply rke.
   + omega.
   + eauto.
 - subst K_x. eapply one_or_empty_of_incl.
 Qed.
 
-Lemma al_in_rkl X `{OrderedType X}
-(s t u : set X) (al : ann (set X)) (x : X) :
-let K :=  of_list (take
-                       (cardinal (t \ s))
-                       (elements (s \ t))
-                  ) in
+Lemma al_in_rkl (s t u : set var) (al : ann (set var)) k :
+let K := kill_oracle (cardinal (t \ s)  - (k - cardinal s)) (s \ t) in
 getAnn al ⊆ s ∪ u ->
  getAnn al
-   [<=] (s \
-         of_list
-           (take (cardinal (t \ s))
-              (elements (s \ t))) ∪ t \ s)
+   [<=] (s \ K ∪ t \ s)
         ∪ (getAnn al ∩ K ∪ u).
 Proof.
-intros K annRM a aIn.
+intros K annRM a aIn. subst K.
 apply union_iff.
-decide (a ∈ of_list (take
-                       (cardinal (t \ s))
-                       (elements (s \ t))
-                    )
-        \/ a ∈ u).
+decide (a ∈ kill_oracle (cardinal (t \ s)  - (k - cardinal s)) (s \ t) \/ a ∈ u).
 - right. cset_tac.
 - left. apply not_or_dist in n. destruct n as [nK nM].
   assert (a ∈ s) as aInR.
   { clear - nM annRM aIn. unfold Subset in annRM.
     specialize (annRM a aIn). cset_tac. }
   cset_tac.
-Qed.
-
-(* move somewhere *)
-Lemma zip_length1
-      (X : Type)
-      (Y : Type)
-      (Z : Type)
-      (f : X -> Y -> Z)
-      (xl: list X)
-      (yl: list Y)
-  :
-    length xl = length yl -> length (f ⊜ xl yl) = length yl
-.
-Proof.
-  intro eq_len.
-  rewrite <- eq_len.
-  apply zip_length2.
-  assumption.
 Qed.
 
 
@@ -302,7 +282,7 @@ Qed.
 
 (**********************************************************************)
 
-Lemma splitSpill_sat_spillSound (k:nat) (s:stmt) (R R' M M': set var)
+Lemma splitSpillKO_sat_spillSound (k:nat) (s:stmt) (R R' M M': set var)
   (Λ Λ': list (set var * set var)) (Lv : list (set var)) (ZL : list params)
   (alv : ann (set var)) :
 R [=] R'
@@ -315,7 +295,7 @@ R [=] R'
 -> PIR2 (fun RMf G => match RMf with (R_f,M_f)
                    => cardinal R_f <= k /\ R_f ∪ M_f ⊆ G end) Λ Lv
 (*-> PIR2 (fun RMf G => fst RMf [=] ∅ /\ snd RMf [=] G) Λ Lv*)
--> spill_sound k ZL Λ (R,M) s (splitSpill k ZL Λ R' M' s alv).
+-> spill_sound k ZL Λ (R,M) s (splitSpillKO k ZL Λ R' M' s alv).
 
 Proof.
 intros ReqR' MeqM' ΛeqΛ' RleqK fvRM fvBound lvSound (*aeFree*) pir2.
@@ -329,153 +309,121 @@ general induction lvSound;
        |k0 Z0 s0 t0 fvBs fvBt];
   (*inversion_clear aeFree;*)
    simpl.
-- assert (rke := @rke var _ R' (Exp.freeVars e) k RleqK fvBcard).
-  assert (fTake := @fTake var _ R' (Exp.freeVars e) (cardinal (Exp.freeVars e \ R'))).
-  set (K := of_list (take
-                       (cardinal (Exp.freeVars e \ R'))
-                       (elements (R' \ Exp.freeVars e))
-                  )) in *.
-  decide (cardinal (R' \ K ∪ Exp.freeVars e \ R') >= k).
-  { rename g into sizeRL.
-    set (K_x:=one_or_empty_if k (R' \ K ∪ Exp.freeVars e \ R' )).
+- assert (RleqK' : cardinal (R' ∩ lv) <= k). {
+    rewrite subset_cardinal. eapply RleqK.
+    clear. cset_tac.
+  }
+  assert (rke := @rke (R' ∩ lv) (Exp.freeVars e) k RleqK' fvBcard).
+  set (K := kill_oracle
+             (cardinal (Exp.freeVars e \ (R' ∩ lv)) - (k - cardinal (R' ∩ lv)))
+             ((R' ∩ lv) \ Exp.freeVars e)
+       ) in *.
 
-    assert (rkk := @rkk var _ R' (Exp.freeVars e) k x).
+  { (*rename g into sizeRL.*)
+    set (K_x:=one_or_empty_if k ((R' ∩ lv) \ K ∪ Exp.freeVars e \ (R' ∩ lv))).
 
+    assert (rkk := @rkk (R' ∩ lv) (Exp.freeVars e) k x).
+    assert (cardinal {x; ((R' ∩ lv) \ K ∪ Exp.freeVars e \ (R' ∩ lv)) \ K_x} <= k). {
+      decide (cardinal
+                ((R' ∩ lv) \
+                           kill_oracle (cardinal (Exp.freeVars e \ (R' ∩ lv))
+                                        - (k - cardinal (R' ∩ lv)))
+                           ((R' ∩ lv) \ Exp.freeVars e) ∪ Exp.freeVars e \ (R' ∩ lv)) < k).
+      - subst K K_x. eauto.
+        rewrite one_or_empty_cardinal_lt; try omega.
+        rewrite add_cardinal.
+        rewrite minus_empty. omega.
+      - eapply rkk; eauto.
+        apply not_ge in n. omega.
+    }
+
+    assert (spill_sound k ZL Λ (R ∩ lv, M) (stmtLet x e s)
+    (ann1 (getAnn al ∩ (K ∪ K_x) \ M', Exp.freeVars e \ (R' ∩ lv), nil)
+       (splitSpillKO k ZL Λ {x; ((R' ∩ lv) \ K ∪ Exp.freeVars e \ (R' ∩ lv)) \ K_x}
+          (getAnn al ∩ (K ∪ K_x) \ M' ∪ M') s al))).
     eapply SpillLet with (K:= K) (Kx := K_x); eauto.
     + subst K K_x; simpl in *.
-      rewrite take_set_incl at 1.
+      rewrite kill_oracle_incl at 1.
       rewrite one_or_empty_of_incl; eauto.
       rewrite Exp.freeVars_live at 4; eauto.
-      rewrite fvRM. rewrite ReqR', MeqM'.
+      revert fvRM.
+      rewrite ReqR', MeqM'.
       clear; cset_tac.
-    + rewrite Exp.freeVars_live; eauto.
-      rewrite fvRM. rewrite ReqR', MeqM'. clear; cset_tac.
+    + rewrite Exp.freeVars_live at 1; eauto.
+      revert fvRM. simpl.
+      rewrite ReqR', MeqM'.
+      clear; cset_tac.
     + eapply IHlvSound;
         try rewrite ReqR'; try rewrite <- MeqM'; try rewrite ΛeqΛ'; eauto.
-      * unfold Subset; intro a. decide (a = x); [cset_tac|].
-        intro aInAnn. rewrite union_iff.
-        (** this can be simplified using al_in_rkl **)
-        decide (   a ∈ K
-              \/ a ∈ K_x
-              \/ a ∈ M
-             ).
-        -- right. revert n aInAnn o; clear; cset_tac.
-        -- left. apply not_or_dist in n0. destruct n0 as [nK nM].
-           decide (a = x).
-           ++ cset_tac.
-           ++ apply add_iff. right.
-              unfold Subset in H0. specialize (H0 a).
-              unfold Subset in fvRM. specialize (fvRM a).
-              assert (a ∈ (getAnn al \ (singleton x))). {
-                revert aInAnn n0; clear; cset_tac.
-              }
-              assert (a ∈ R'). {
-                rewrite <- ReqR'.
-                revert nM H3 H0 fvRM. clear; cset_tac.
-              }
-              assert (a ∈ R' \ K). {
-                revert H4 nK; clear; cset_tac.
-              }
-              revert nM H5; clear; cset_tac.
-    + rewrite ReqR'. apply fTake.
+      * simpl in *.
+        eapply Exp.freeVars_live in H; eauto.
+        revert H0 fvRM H.
+        rewrite ReqR'.
+        clear. clearbody K K_x. cset_tac'.
+    + rewrite ReqR'. apply kill_oracle_incl2.
     + rewrite ReqR'. apply rke.
 
-    + rewrite ReqR'. apply rkk; eauto.
+    + rewrite ReqR'; eauto.
+    + eapply spill_sound_incl_R; eauto.
+      * clear; cset_tac.
+      * rewrite ReqR'. eauto.
   }
 
-  {
-  rename n into sizeRL.
-
-
-  assert (cardinal (Exp.freeVars e) < k) as leqK.
-  { apply not_ge in sizeRL.
-    rewrite <- fTake in sizeRL. exact sizeRL. }
-
-  eapply SpillLet with
-            (K:= of_list (take
-                            (cardinal (Exp.freeVars e \ R'))
-                            (elements (R' \ Exp.freeVars e))
-                          )
-            )
-              (Kx := ∅).
-  + subst K; simpl in *.
-    rewrite take_set_incl at 1.
-    rewrite one_or_empty_of_incl; eauto.
-    rewrite Exp.freeVars_live at 4; eauto.
-    rewrite fvRM. rewrite ReqR', MeqM'.
-    clear; cset_tac.
-  + rewrite Exp.freeVars_live at 1; eauto.
-    rewrite fvRM. rewrite ReqR', MeqM'. clear; cset_tac.
-  + eapply IHlvSound; eauto.
-    * rewrite one_or_empty_cardinal_lt; try omega.
-      subst K. rewrite ReqR'. cset_tac.
-    * rewrite MeqM'. cset_tac.
-    * rewrite one_or_empty_cardinal_lt; try omega.
-      clear - sizeRL. rewrite add_cardinal. apply not_ge in sizeRL.
-      rewrite minus_empty. omega.
-    * rewrite ReqR', MeqM'. simpl in *. rewrite fvRM in H0.
-      rewrite ReqR', MeqM' in H0.
-      clear - sizeRL H0 fvRM ReqR' MeqM'.
-      rewrite one_or_empty_cardinal_lt; try omega.
-      unfold Subset; intro a. decide (a === x); [cset_tac|].
-        intro aInAnn. rewrite union_iff.
-        (** this can be simplified using al_in_rkl **)
-        decide (   a ∈ K
-              \/ a ∈ M'
-             ).
-      -- right. revert aInAnn o. clear. cset_tac.
-      -- refold. clearbody K.
-         revert aInAnn n0 n H0. clear; cset_tac.
-  + rewrite ReqR'. eauto.
-  + eauto.
-  + subst K... rewrite ReqR'. exact rke.
-  + rewrite minus_empty. rewrite add_cardinal. apply not_ge in sizeRL.
-    rewrite ReqR'. clear - sizeRL. subst K... omega.
-  }
-- set (K := of_list (take
-                       (cardinal (Op.freeVars e \ R'))
-                       (elements (R' \ Op.freeVars e))
-                  )) in *.
+- rewrite <- ReqR' in RleqK.
+  assert (Incl:R' ∩ lv ⊆ R) by (rewrite ReqR'; clear; cset_tac).
+  assert (Card:cardinal (R' ∩ lv) <= k) by (rewrite Incl; eauto).
+  eapply spill_sound_incl_R with (R:=R' ∩ lv); eauto.
+  set (K := kill_oracle (cardinal (Op.freeVars e \ (R' ∩ lv)) - (k - cardinal (R' ∩ lv)))
+                       ((R' ∩ lv) \ Op.freeVars e)) in *.
   eapply SpillIf with (K:= K);
-  [  |  | rewrite ReqR'; apply fTake
-  | rewrite ReqR'; apply rke; eauto
+  [  |  | apply kill_oracle_incl2
+  | apply rke; eauto
   | eapply IHlvSound1
-  | eapply IHlvSound2 ];
-  try rewrite ReqR'; try rewrite <- MeqM'; eauto;
-  [ | | apply rke ; eauto  | | apply rke; eauto | ];
-  [ | | rewrite <- seteq_1 | rewrite <- seteq_2 ];
-  try (subst K; apply al_in_rkl; eauto;
-       rewrite <- ReqR'; eauto with cset).
-  simpl in *. subst K.
-  rewrite take_set_incl. clear; cset_tac.
-  rewrite Op.freeVars_live; eauto. simpl in *.
-  rewrite fvRM. rewrite ReqR'. clear; cset_tac.
-- eapply PIR2_nth_2 with (l:=counted l) in pir2; eauto using zip_get.
+  | eapply IHlvSound2 ]; eauto;
+    try rewrite ReqR'; try rewrite MeqM';
+      try eapply rke; eauto.
+  + subst K. rewrite kill_oracle_incl. clear; cset_tac.
+  + rewrite Op.freeVars_live; eauto.
+    simpl in *. revert fvRM. rewrite ReqR', MeqM'.
+    clear; cset_tac.
+  + subst K.
+    rewrite (@al_in_rkl (R' ∩ lv) (Op.freeVars e) M' _ k) at 1.
+    clear. cset_tac. revert fvRM H0; simpl; rewrite ReqR', MeqM'.
+    clear. cset_tac.
+  + subst K.
+    rewrite (@al_in_rkl (R' ∩ lv) (Op.freeVars e) M' _ k) at 1.
+    clear. cset_tac. revert fvRM H1; simpl; rewrite ReqR', MeqM'.
+    clear. cset_tac.
+- assert (InclR':R' ∩ lv ⊆ R) by (rewrite ReqR'; clear; cset_tac).
+  eapply spill_sound_incl_R with (R:=R' ∩ lv); [ | |rewrite ReqR'];eauto.
+  eapply PIR2_nth_2 with (l:=counted l) in pir2; eauto using zip_get.
   destruct pir2 as [[R_f M_f] [pir2_get [pir2_R1 pir2_R2]]]. simpl in *.
   repeat erewrite get_nth; eauto; simpl.
-  assert (Incl:(R_f ∪ M_f) \ of_list Z [<=] blv \ of_list Z).
-  rewrite <- pir2_R2; eauto.
-  set (K := of_list (take
-                      (cardinal ((R_f \ R') \ of_list Z))
-                      (elements (R' \ R_f))
-                     )) in *.
+  assert (Incl:(R_f ∪ M_f) \ of_list Z [<=] blv \ of_list Z). {
+    rewrite <- pir2_R2; eauto.
+  }
+  set (K := kill_oracle
+             (cardinal ((R_f \ (R' ∩ lv)) \ of_list Z) - (k - cardinal (R' ∩ lv)))
+             ((R' ∩ lv) \ R_f)) in *.
   eapply SpillApp with (K:= K); try rewrite ReqR'; try rewrite MeqM'; eauto.
   + subst K.
     rewrite Op.freeVars_live_list; eauto.
-    rewrite take_set_incl.
-    rewrite fvRM. rewrite ReqR', MeqM'.
-    rewrite H1, fvRM in Incl. revert Incl.
+    rewrite (@kill_oracle_incl _ kos).
+    rewrite H1 in Incl.
+    revert fvRM Incl.
     rewrite ReqR', MeqM'.
     clear; cset_tac.
   + rewrite H1, fvRM in Incl. revert Incl.
     rewrite ReqR', MeqM'.
-    clear; cset_tac.
+    rewrite <- pir2_R2 in H1. revert H1.
+    clear; cset_tac'.
   + subst K.
-    eauto using rke'.
-  + rewrite <- minus_incl with (s:=R'\K) (t:=of_list Z).
+    eapply rke'; eauto. rewrite InclR'; eauto. rewrite ReqR'; eauto.
+  + rewrite <- minus_incl with (s:=(R' ∩ lv)\K) (t:=of_list Z).
     rewrite minus_union_minus.
-    apply incl_minus_lr with (s:=R_f) (s':=R'\K ∪ R_f \ R') (t:=of_list Z) (t':=of_list Z).
-    * subst K. eapply fTake.
+    apply incl_minus_lr with (s:=R_f) (s':=(R' ∩ lv)\K ∪ R_f \ (R' ∩ lv))
+                                      (t:=of_list Z) (t':=of_list Z).
+    * subst K. eapply kill_oracle_incl2.
     * eauto.
   + clearbody K. clear_all. cset_tac.
   + subst K.
@@ -485,22 +433,24 @@ general induction lvSound;
                              ∪ (R_f \ R') \ of_list Z)).
     * revert i. clear_all. cset_tac.
     * revert n. clear_all. cset_tac.
-  + edestruct @list_eq_get; eauto; dcr. destruct x as [R_f' M_f']; invc H6.
-    repeat erewrite get_nth; eauto; simpl.
-    rewrite H1, fvRM, ReqR', MeqM' in Incl.
-    exploit Op.freeVars_live_list; eauto. rewrite fvRM in H4.
-    rewrite ReqR' in H4. rewrite MeqM' in H4.
-    revert H4. clear. clearbody K. cset_tac.
-- set (K := of_list (take
-                       (cardinal (Op.freeVars e \ R'))
-                       (elements (R' \ Op.freeVars e))
-                  )) in *.
+  + edestruct @list_eq_get; eauto; dcr.
+    destruct x as [R_f' M_f']; invc H6.
+    rewrite <- pir2_R2 in H1.
+    exploit Op.freeVars_live_list; eauto.
+    revert H1 H4 fvRM. rewrite ReqR'. rewrite MeqM'.
+    clear. clearbody K. cset_tac.
+- assert (InclR':R' ∩ lv ⊆ R) by (rewrite ReqR'; clear; cset_tac).
+  eapply spill_sound_incl_R with (R:=R' ∩ lv); [ | |rewrite ReqR'];eauto.
+
+  set (K := kill_oracle (cardinal (Op.freeVars e \ (R' ∩ lv)) - (k - cardinal (R' ∩ lv)))
+                       ((R' ∩ lv)\ Op.freeVars e)) in *.
   eapply SpillReturn with (K:= K); try rewrite ReqR'; eauto.
   + clear_all. cset_tac.
   + rewrite Op.freeVars_live; eauto.
-    rewrite <- ReqR'. rewrite fvRM. cset_tac.
-  + apply fTake.
-  + apply rke; eauto.
+    rewrite <- ReqR'. revert fvRM. simpl. clear. cset_tac.
+  + apply kill_oracle_incl2.
+  + apply rke; eauto. rewrite <- RleqK.
+    eapply subset_cardinal. cset_tac.
 - eapply SpillFun with (K:=∅); eauto.
   + clear. cset_tac.
   + assert (forall s:set var, s \ ∅ ∪ ∅ [=] s) as seteq'. {
@@ -508,11 +458,8 @@ general induction lvSound;
       cset_tac.
     }
     rewrite (seteq' R). rewrite ReqR'. apply RleqK.
-  + symmetry. apply zip_length2. rewrite H.
-    symmetry. apply zip_length1.
-    apply zip_length1.
-    assumption.
-  + symmetry. apply zip_length2. assumption.
+  + eauto with len.
+  + eauto with len.
   + intros ; inv_get. simpl. apply take_of_list_cardinal.
   + intros ; inv_get.
     eapply H1; eauto.
@@ -526,9 +473,6 @@ general induction lvSound;
          clear; eauto with cset.
   + eapply IHlvSound; eauto.
     * rewrite ReqR'. clear. cset_tac.
-   (* * (8 apply list_eq_app.
-      -- reflexivity.
-      -- apply ΛeqΛ'. *)
     * rewrite H3. simpl in fvRM. rewrite fvRM. clear. cset_tac.
     * eapply PIR2_app; eauto.
       eapply PIR2_get; eauto with len.
@@ -540,10 +484,10 @@ general induction lvSound;
 Qed.
 
 
-Lemma splitSpill_spill_live VD k ZL Lv Λ R M s alv
+Lemma splitSpillKO_spill_live VD k ZL Lv Λ R M s alv
       (LS:live_sound Imperative ZL Lv s alv)
       (lvIncl:ann_P (fun lv => lv ⊆ VD) alv)
-  : spill_live VD (splitSpill k ZL Λ R M s alv) alv.
+  : spill_live VD (splitSpillKO k ZL Λ R M s alv) alv.
 Proof.
   move s before k.
   revert_until s.
@@ -558,3 +502,18 @@ Proof.
       exploit H7; eauto. eapply ann_P_get in H4. rewrite <- H4.
       rewrite take_set_incl at 1; simpl; eauto 20 with cset.
 Qed.
+
+
+Instance taken_kos : kill_oracle_spec (@set_take var _).
+Proof.
+  econstructor; intros;
+    eauto using set_take_cardinal_eq, set_take_eq, set_take_incl.
+  eapply set_take_eq; eauto. omega.
+Qed.
+
+End KO.
+
+Definition splitSpill := @splitSpillKO (@set_take var _).
+
+Definition splitSpill_sat_spillSound := @splitSpillKO_sat_spillSound _ taken_kos.
+Definition splitSpill_spill_live := @splitSpillKO_spill_live (@set_take var _).
