theories/Spilling/SpillSoundFive.v
@@ -2,129 +2,6 @@ Require Import List Map Env AllInRel Exp.
 Require Import IL Annotation AnnP InRel.
 Require Import LabelsDefined SpillSound SpillUtil.
 
-Lemma list_eq_PIR2 X `{OrderedType X} (L L':list X)
-  : L === L'
-    -> PIR2 _eq L L'.
-Proof.
-  intros. general induction H0; eauto using PIR2.
-Qed.
-
-Lemma spill_sound_ext
-      (k : nat)
-      (ZL : list params) s
-      (Λ Λ2 : list (⦃var⦄ * ⦃var⦄))
-      (R R2 M M2 : ⦃var⦄)
-      (sl sl2 : spilling)
-  :
-    PIR2 _eq Λ Λ2
-    -> R [=] R2
-    -> M [=] M2
-    -> sl === sl2
-    -> spill_sound k ZL Λ (R,M) s sl -> spill_sound k ZL Λ2 (R2,M2) s sl2
-.
-Proof.
-  intros Λeq Req Meq sleq H.
-  general induction H; simpl; eauto.
-    destruct sl2; isabsurd;
-      destruct a as [[Sp' L'] rm'].
-  - destruct rm'; [|clear - sleq; invc sleq; invc H2; isabsurd].
-    eapply SpillLet with (K:=K) (Kx:=Kx); simpl; eauto; invc sleq; invc H9; invc H10.
-    + rewrite <-Req, <-H9. assumption.
-    + rewrite <-Meq, <-H14, <-H9. assumption.
-    + eapply IHspill_sound; eauto.
-      * rewrite Req, H14; clear; cset_tac.
-      * rewrite H9, Meq; clear; cset_tac.
-    + rewrite <-Req, <-H14; assumption.
-    + rewrite <-Req, <-H14; assumption.
-    + rewrite <-Req, <-H14; assumption.
-  - invc sleq. invc H4.
-    inv H8. inv H6. econstructor; eauto.
-    rewrite <- H5. rewrite <- Req. eauto.
-    rewrite <- H5, <- H9. rewrite <- Meq. eauto.
-    rewrite <- H9. rewrite <- Req. eauto.
-    rewrite <- Req, <- H9. eauto.
-  - inv sleq. inv H8. inv H7; invc H12.
-    eapply SpillIf with (K:=K).
-    + rewrite <-H9, <-Req. assumption.
-    + rewrite <-Meq, <-H9, <-H14; assumption.
-    + rewrite <-Req, <-H14; assumption.
-    + rewrite <-Req, <-H14; assumption.
-    + eapply IHspill_sound1; eauto.
-      * rewrite Req, H14; clear; cset_tac.
-      * rewrite Meq, H9; clear; cset_tac.
-    + eapply IHspill_sound2; eauto.
-      * rewrite Req, H14; clear; cset_tac.
-      * rewrite Meq, H9; clear; cset_tac.
-  - PIR2_inv.
-    invc sleq. invc H10. invc H16. invc H17.
-    invc H14. invc H12.
-    eapply SpillApp with (K:=K); eauto.
-    + rewrite <- H15, <- Req; eauto.
-    + rewrite <- H15, <- H17, <- Meq; eauto.
-    + rewrite <- H17, <- Req; eauto.
-    + rewrite <- H11, <- Req, <- H17; eauto.
-    + rewrite <- H13, <- Meq, <- H15; eauto.
-    + rewrite <- H18, <- Req, <- H17; eauto.
-    + rewrite <- H18, <- Meq, <- H15; eauto.
-  - invc sleq. invc H11. invc H10.
-    eapply SpillFun with (K:=K); eauto.
-    + rewrite <- H11, <- Req; eauto.
-    + rewrite <- H11, <- H17, <- Meq; eauto.
-    + rewrite <- H17, <- Req. eauto.
-    + eauto with len.
-    + hnf in H16. eapply list_eq_length in H16. eauto with len.
-    + intros. symmetry in H16.
-      edestruct @list_eq_get; try eapply H16; eauto; dcr.
-      exploit H4; eauto. rewrite H13. eauto.
-    + intros. inv_get.
-      exploit H14; eauto.
-      edestruct @list_eq_get; try eapply H16; eauto; dcr.
-      inv_get. invc H22.
-      eapply H6; eauto.
-      * eapply PIR2_app; eauto using list_eq_PIR2.
-      * eapply H20.
-      * eapply H21.
-    + eapply IHspill_sound; eauto.
-      * eapply PIR2_app; eauto using list_eq_PIR2.
-      * rewrite <- Req, <- H17. eauto.
-      * rewrite <- H11. rewrite <- Meq. eauto.
-Qed.
-
-Instance spill_sound_morphX k ZL Λ
-  : Proper (_eq ==> eq ==> @equiv _ _ _ ==> iff) (spill_sound k ZL Λ).
-Proof.
-  unfold Proper, respectful; intros; subst; split; intros; inv H.
-  - eapply spill_sound_ext; eauto; try reflexivity.
-    eapply H2. eapply H3.
-  - eapply spill_sound_ext; try eapply H0; try reflexivity.
-    rewrite H2; eauto. rewrite H3; eauto. symmetry; eauto.
-Qed.
-
-Instance spill_sound_morph_implX k ZL Λ
-  : Proper (_eq ==> eq ==> @equiv _ _ _ ==> impl) (spill_sound k ZL Λ).
-Proof.
-  unfold Proper, respectful, impl; intros; subst; intros; inv H.
-  - eapply spill_sound_ext; try eapply H2; try reflexivity.
-    rewrite H0; eauto. rewrite H3; eauto. symmetry; eauto.
-Qed.
-
-Instance spill_sound_morph_flip_implX k ZL Λ
-  : Proper (_eq ==> eq ==> @equiv _ _ _ ==> flip impl) (spill_sound k ZL Λ).
-Proof.
-  unfold Proper, respectful, flip, impl; intros; subst; intros; inv H.
-  - eapply spill_sound_ext; try eapply H2; try reflexivity.
-    rewrite H0; eauto. rewrite H3; eauto. symmetry; eauto.
-Qed.
-
-Instance spill_sound_morphX' k ZL Λ
-  : Proper (@pe _ _ ==> eq ==> @equiv _ _ _ ==> iff) (spill_sound k ZL Λ).
-Proof.
-  unfold Proper, respectful; intros; subst; split; intros; inv H.
-  - eapply spill_sound_ext; eauto; try reflexivity.
-  - eapply spill_sound_ext; try eapply H0; try reflexivity.
-    rewrite H2; eauto. rewrite H3; eauto. symmetry; eauto.
-Qed.
-
 
 Inductive spill_sound (k:nat) :
   (list params)
@@ -239,6 +116,7 @@ Smpl Add
      end : inv_trivial.
 
 
+
 Instance clear_Sp_morph
   : Proper (@equiv _ (ann_R _eq) _ ==> equiv) clear_Sp.
 Proof.
@@ -268,7 +146,6 @@ Proof.
   * econstructor; eauto;
       rewrite H3; reflexivity.
 Qed.
-
 
 Lemma spill_sound_ext'
       (k : nat)
@@ -369,123 +246,6 @@ Proof.
   - eapply spill_sound_ext'; eauto; try reflexivity.
   - eapply spill_sound_ext'; try eapply H0; try reflexivity.
     rewrite H2; eauto. rewrite H3; eauto. symmetry; eauto.
-Qed.
-
-
-Lemma spill_sound_spill_ext k ZL Λ (R0 M0:set var) s sl
-  (SPS: SpillSound.spill_sound k ZL Λ (R0, getSp sl ∪ M0) s (clear_Sp sl))
-  (Sp_sub : getSp sl [<=] R0)
-  (Rsmall : cardinal R0 <= k)
-  : SpillSound.spill_sound k ZL Λ (R0, M0) s sl.
-Proof.
-  destruct sl; invc SPS; simpl in *; clear_trivial_eqs.
-  - destruct p. econstructor; eauto.
-  - simpl in *. destruct p. econstructor; eauto.
-  - destruct p; simpl in *. econstructor; eauto.
-    set_simpl. eauto.
-  - destruct p; simpl in *. set_simpl.
-    econstructor; eauto.
-  - destruct a. destruct p.
-    econstructor; eauto.
-    simpl in *. set_simpl. eauto.
-Qed.
-
-Lemma spill_sound_incl_R k ZL Λ R R' s sl M
-  (SPS:SpillSound.spill_sound k ZL Λ (R,M) s sl)
-  (Incl: R ⊆ R')
-  (Card:cardinal R' <= k)
-  : SpillSound.spill_sound k ZL Λ (R',M) s sl.
-Proof.
-  destruct sl; invc SPS; simpl in *.
-  - eapply SpillSound.SpillReturn with (K:=K ∪ R' \ R); eauto with cset.
-    + rewrite H7.
-      revert Incl; clear_all; cset_tac.
-    + rewrite <- H8. eapply subset_cardinal.
-      revert Incl; clear_all; cset_tac.
-  - eapply SpillSound.SpillApp with (K:=K ∪ R' \ R); eauto.
-    + eauto with cset.
-    + rewrite <- H4. eapply subset_cardinal.
-      revert Incl; clear_all; cset_tac.
-    + rewrite H7.
-      revert Incl; clear_all; cset_tac.
-    + rewrite H12.
-      revert Incl; clear_all; cset_tac.
-  - eapply SpillSound.SpillLet with (K:=K ∪ R' \ R); eauto.
-    + eauto with cset.
-    + assert ({x; (R' \ (K ∪ R' \ R) ∪ L) \ Kx}
-                [=] {x; (R \ K ∪ L) \ Kx}). {
-        revert Incl; clear_all; cset_tac.
-      }
-      rewrite H. eauto.
-    + rewrite H8.
-      revert Incl; clear_all; cset_tac.
-    + rewrite <- H11. eapply subset_cardinal.
-      revert Incl; clear_all; cset_tac.
-    + rewrite <- H12. eapply subset_cardinal.
-      revert Incl; clear_all; cset_tac.
-  - assert (EQ:R' \ (K ∪ R' \ R) ∪ L
-              [=] R \ K ∪ L). {
-      revert Incl; clear_all; cset_tac.
-    }
-    eapply SpillSound.SpillIf with (K:=K ∪ R' \ R); eauto;
-                                try rewrite EQ; eauto with cset.
-  - assert (EQ:R' \ (K ∪ R' \ R) ∪ L
-              [=] R \ K ∪ L). {
-      revert Incl; clear_all; cset_tac.
-    }
-    eapply SpillSound.SpillFun with (K:=K ∪ R' \ R); eauto;
-                                try rewrite EQ; eauto.
-    + eauto with cset.
-Qed.
-
-Lemma spill_sound_load_ext k ZL Λ (R0 M0:set var) Ka s sl
-      (card:cardinal R0 <= k)
-      (card2: cardinal (R0 \ Ka ∪ getL sl) <= k)
-      (SPS: SpillSound.spill_sound k ZL Λ (R0 \ Ka ∪ getL sl, M0) s (clear_L sl))
-      (L_sub : getL sl [<=] M0)
-      (SpE:getSp sl [=] ∅)
-  : SpillSound.spill_sound k ZL Λ (R0, M0) s sl.
-Proof.
-  destruct sl; inv SPS; simpl in *; clear_trivial_eqs;
-    try destruct p as [Sp L]; simpl in *.
-  - eapply SpillSound.SpillReturn with (K:=Ka).
-    + rewrite SpE. eauto with cset.
-    + rewrite L_sub. eauto with cset.
-    + rewrite H9. set_simpl. cset_tac.
-    + eauto.
-  - econstructor; eauto.
-    + rewrite SpE. eauto with cset.
-    + rewrite L_sub. eauto with cset.
-    + rewrite H12. clear; cset_tac.
-    + rewrite H14. clear; cset_tac.
-  - econstructor; eauto.
-    + rewrite SpE. eauto with cset.
-    + rewrite L_sub. eauto with cset.
-    + set_simpl. instantiate (1:=K ∪ Kx).
-      rewrite <- minus_union. eauto.
-    + rewrite H11. clear; cset_tac.
-    + rewrite <- H14.
-      eapply subset_cardinal.
-      clear_all. cset_tac'.
-  - eapply SpillSound.SpillIf with (K:=K ∪ Ka).
-    + rewrite SpE. eauto with cset.
-    + rewrite L_sub. eauto with cset.
-    + rewrite H11. clear_all. cset_tac.
-    + rewrite <- card2. eapply subset_cardinal. clear; cset_tac.
-    + eapply spill_sound_incl_R; eauto.
-      * clear; cset_tac.
-      * rewrite <- card2. eapply subset_cardinal.
-        clear; cset_tac.
-    + eapply spill_sound_incl_R; eauto.
-      * clear; cset_tac.
-      * rewrite <- card2. eapply subset_cardinal.
-        clear; cset_tac.
-  - destruct a, p; simpl in *.
-    econstructor; eauto.
-    + rewrite SpE; eauto with cset.
-    + rewrite L_sub; eauto with cset.
-    + eapply spill_sound_incl_R; eauto.
-      * clear; cset_tac.
 Qed.
 
 Lemma spill_sound_spill_sound3
